Persistence: non-trivial fixes
These are (some) changes to lty, path_wp, ds_unary_lr, unary_lr,
no_russell_paradox, sem_kind, which aren't just a matter of dropping
persistence.

theories/iris_extra/lty.v
@@ -36,15 +36,13 @@ https://gitlab.mpi-sws.org/iris/examples/blob/d4f4153920ea82617c7222aeeb00b6710d
 
 Record iPPred vl Σ := IPPred {
   iPPred_car :> vl → iProp Σ;
-  iPPred_persistent v : Persistent (iPPred_car v);
 }.
 Add Printing Constructor iPPred.
-Global Arguments IPPred {_ _} _%I {_}.
+Global Arguments IPPred {_ _} _%I.
 Global Arguments iPPred_car {_ _} !_ _ /.
 Declare Scope iPPred_scope.
 Bind Scope iPPred_scope with iPPred.
 Delimit Scope iPPred_scope with T.
-Global Existing Instance iPPred_persistent.
 
 (** ** OFE on [iPPred]. *)
 Section iPPred_ofe.
@@ -68,19 +66,10 @@ Section iPPred_ofe.
   (** ** Show iPPred forms a COFE.
   Only needed to define Lty using Iris fixpoints (e.g. for normal recursive
   types), so _currently_ unused. *)
-  Definition pred_persistent (A : vl -d> iPropO Σ) := ∀ w, Persistent (A w).
-
-  Instance: LimitPreserving pred_persistent.
-  Proof.
-    apply limit_preserving_forall=> v.
-    apply bi.limit_preserving_Persistent => n f g Heq. exact: Heq.
-  Qed.
 
   Global Instance iPPred_cofe : Cofe iPPredO.
   Proof.
-    apply (iso_cofe_subtype' pred_persistent IPPred lApp) => //.
-    - by move => [].
-    - apply _.
+    apply (iso_cofe (A := vl -d> iPropO Σ) IPPred lApp) => //.
   Qed.
 
   Global Instance bottom_iprop : Bottom (iProp Σ) := False%I.
@@ -96,14 +85,9 @@ Section iPPred_ofe.
   Global Instance iPPred_car_proper : Proper ((≡) ==> (=) ==> (≡)) (@iPPred_car vl Σ).
   Proof. by intros A A' HA w ? <-. Qed.
 
-  (*
-    Since substitution lemmas don't use setoids,
-    [HSubstLemmas vl (olty Σ i)] requires proof irrelevance.
-   *)
   Lemma lty_eq τ1 τ2: iPPred_car τ1 = iPPred_car τ2 → τ1 = τ2.
   Proof.
-    move: τ1 τ2 => [φ1 Hp1] [φ2 Hp2]. rewrite /iPPred_car.
-    intros ->. f_equal; exact: ProofIrrelevance.proof_irrelevance.
+    move: τ1 τ2 => [φ1 ] [φ2 ] /=. by rewrite /iPPred_car => ->.
   Qed.
 End iPPred_ofe.
 
@@ -121,7 +105,7 @@ Notation lty_car := (iPPred_car (vl := vl)) (only parsing).
 Notation lApp := (iPPred_car : lty _ → _ -d> _).
 
 Notation iRel P Σ := (P Σ → P Σ → iProp Σ).
-Definition subtype_lty {Σ} : iRel ltyO Σ := λI φ1 φ2,
+Definition subtype_lty `{dlangG Σ} : iRel ltyO Σ := λI φ1 φ2,
   ∀ v, φ1 v → φ2 v.
 Infix "⊆" := subtype_lty : bi_scope.
 Notation "X ⊆@{ Σ } Y" := (subtype_lty (Σ := Σ) X Y) (at level 70, only parsing) : bi_scope.
@@ -129,7 +113,7 @@ Notation "X ⊆ Y ⊆ Z" := (X ⊆ Y ∧ Y ⊆ Z)%I : bi_scope.
 Notation "X ⊆ Y ⊆ Z ⊆ W" := (X ⊆ Y ∧ Y ⊆ Z ∧ Z ⊆ W)%I (at level 70, Y, Z at next level) : bi_scope.
 
 Section subtype_lty.
-  Context {Σ}.
+  Context `{dlangG Σ}.
 
   Global Instance subtype_lty_ne : NonExpansive2 (subtype_lty (Σ := Σ)).
   Proof. solve_proper_ho. Qed.
@@ -177,7 +161,7 @@ Instance packHoLtyO_proper {Σ n} :
 
 (** ** Substitution over [olty]. *)
 Section olty_subst.
-  Context `{Σ : gFunctors} {i : nat}.
+  Context `{dlangG Σ} {i : nat}.
   Implicit Types (φ : hoEnvD Σ i) (τ : olty Σ i).
 
   Lemma olty_eq τ1 τ2:
